\documentclass[fleqn,12pt]{article}
\newcommand{\expectation}[1]{\langle #1 \rangle}
\begin{document}
\title{Statistical Function Notes}
\author{Brian Gough}
\date{November 2008}
\maketitle

\section{Weighted mean and variance}
We have $N$ samples $x_i$ drawn from a gaussian distribution
$G(\mu,\sigma)$.  Each sample has a weight $w_i$ which represents the
relative value we place on it.  Given the estimate of the mean
%
\begin{eqnarray}
\bar{x} &=& {1 \over W} \sum_i w_i x_i \\
W       &=& \sum_i w_i
\end{eqnarray}
%
\noindent
we want an unbiased estimator of the variance of the underlying
distribution $\sigma^2$.  

We start with the standard definition of the sample variance $V$ and
compute the bias correction factor.
%
\begin{eqnarray}
V &=& {1\over W} \sum_i w_i (x_i - \bar{x})^2 \\
  &=& {1\over W} \sum_i w_i \left(x_i - {1\over W}\sum_j w_j x_j\right)^2 \\
  &=& {1\over W} \sum_i w_i \left(x_i^2 - {2 \over W} x_i \sum_j w_j x_j 
       + {1 \over W^2} (\sum_j w_j x_j)^2\right) \\
  &=& {1\over W} \left( \sum_i w_i x_i^2 
       - {2 \over W} \sum_i w_i x_i \sum_j w_j x_j
       + {1 \over W} (\sum_j w_j x_j)^2\right)\\
  &=& {1\over W} \left( \sum_i w_i x_i^2 
       - {1 \over W} \sum_i w_i x_i \sum_j w_j x_j\right)\\
  &=& {1\over W} \left( \sum_i w_i x_i^2 
       - {1 \over W} \sum_{ij} w_i w_j x_i x_j\right)
\end{eqnarray}
%
We find the expectation value $\expectation{V}$ using the Gaussian formulas
$\expectation{x_i} = \mu$, $\expectation{x_i x_j} = \mu^2 + \delta_{ij} \sigma^2$.
%
\begin{eqnarray}
\expectation{V}   &=& {1\over W} \left( \sum_i w_i \expectation{x_i^2}
       - {1 \over W} \sum_{ij} w_i w_j \expectation{x_i x_j}\right)\\
      &=& {1\over W} \left( \sum_i w_i (\mu^2 + \sigma^2)
       - {1 \over W} \sum_{ij} w_i w_j (\mu^2 + \delta_{ij} \sigma^2)\right)\\
      &=& {1\over W} \left( W (\mu^2 + \sigma^2)
       - {1 \over W} ( W^2 \mu^2 +( \sum_i w_i^2) \sigma^2)\right)\\
      &=& {1\over W} \left(W - {1 \over W} ( \sum_i w_i^2)\sigma^2\right)\\
      &=& \left({{W^2 - \sum_i w_i^2} \over W^2}\right) \sigma^2
\end{eqnarray}
%
Therefore an unbiased estimator $U$ of $\sigma^2$ is
%
\begin{eqnarray}
U &=& {W^2 \over {(W^2 - \sum_i w_i^2)}} \expectation{V}\\
  &=& {W^2 \over {(W^2 - \sum_i w_i^2)}} {1\over W} \sum_i w_i (x_i - \bar{x})^2 \\
  &=& {W \over {(W^2 - \sum_i w_i^2)}} \sum_i w_i (x_i - \bar{x})^2
\end{eqnarray}
%
And this is the formula used in GSL.
\subsection{Notes}
Note the following properties:

\begin{itemize}
\item
The formula is invariant under rescaling of the weights.

\item 
For equal weights $w_i = w$ the factor reduces to $N/(N^2-N) =
1/(N-1)$, which is the familiar factor of the unbiased estimator of
the variance for data without weights.

\item
When $\sum_i (w_i/W)^2 \ll 1$ the commonly-used weighted variance
formula $V = (1/W)\sum_i w_i (x_i - \bar{x})^2$ is a good
approximation.
\end{itemize}
\end{document}

